Prefix(:=<http://www.ease-crc.org/ont/SOMA-IO.owl#>)
Prefix(dc:=<http://purl.org/dc/elements/1.1/>)
Prefix(owl:=<http://www.w3.org/2002/07/owl#>)
Prefix(rdf:=<http://www.w3.org/1999/02/22-rdf-syntax-ns#>)
Prefix(xml:=<http://www.w3.org/XML/1998/namespace>)
Prefix(xsd:=<http://www.w3.org/2001/XMLSchema#>)
Prefix(SOMA:=<http://www.ease-crc.org/ont/SOMA.owl#>)
Prefix(rdfs:=<http://www.w3.org/2000/01/rdf-schema#>)


Ontology(<http://www.ease-crc.org/ont/SOMA-PYCRAM.owl>
Import(<http://www.ease-crc.org/ont/SOMA-ALL.owl>)

Declaration(Class(<http://www.ease-crc.org/ont/SOMA-PYCRAM.owl#PyCramActionDesignatorDescription>))
Declaration(Class(<http://www.ease-crc.org/ont/SOMA-PYCRAM.owl#PyCramActionDesignatorReferenet>))
Declaration(Class(<http://www.ease-crc.org/ont/SOMA-PYCRAM.owl#PyCramDesignatorDescription>))
Declaration(Class(<http://www.ease-crc.org/ont/SOMA-PYCRAM.owl#PyCramDesignatorReferent>))
Declaration(Class(<http://www.ease-crc.org/ont/SOMA-PYCRAM.owl#PyCramLocationDesignator>))
Declaration(Class(<http://www.ease-crc.org/ont/SOMA-PYCRAM.owl#PyCramLocationDesignatorDescription>))
Declaration(Class(<http://www.ease-crc.org/ont/SOMA-PYCRAM.owl#PyCramLocationDesignatorReferenet>))
Declaration(Class(<http://www.ease-crc.org/ont/SOMA-PYCRAM.owl#PyCramMotionDesignatorDescription>))
Declaration(Class(<http://www.ease-crc.org/ont/SOMA-PYCRAM.owl#PyCramMotionDesignatorReferenet>))
Declaration(Class(<http://www.ease-crc.org/ont/SOMA-PYCRAM.owl#PyCramObjectDesignatorDescription>))
Declaration(Class(<http://www.ease-crc.org/ont/SOMA-PYCRAM.owl#PyCramObjectDesignatorReferenet>))
Declaration(Class(SOMA:PyCramActionDesignator))
Declaration(Class(SOMA:PyCramDesignator))
Declaration(Class(SOMA:PyCramMotionDesignator))
Declaration(Class(SOMA:PyCramObjectDesignator))
Declaration(Class(SOMA:Resolving_of_PyCRAM_Designators))



############################
#   Classes
############################

# Class: <http://www.ease-crc.org/ont/SOMA-PYCRAM.owl#PyCramActionDesignatorDescription> (PyCRAM Action Designator Description)

AnnotationAssertion(rdfs:comment <http://www.ease-crc.org/ont/SOMA-PYCRAM.owl#PyCramActionDesignatorDescription> "Expresses an (underspecified) description (dul:Description) used by the CRAM framework to resolve actions at runtime.")
AnnotationAssertion(rdfs:label <http://www.ease-crc.org/ont/SOMA-PYCRAM.owl#PyCramActionDesignatorDescription> "PyCRAM Action Designator Description")
SubClassOf(<http://www.ease-crc.org/ont/SOMA-PYCRAM.owl#PyCramActionDesignatorDescription> <http://www.ease-crc.org/ont/SOMA-PYCRAM.owl#PyCramDesignatorDescription>)
SubClassOf(<http://www.ease-crc.org/ont/SOMA-PYCRAM.owl#PyCramActionDesignatorDescription> ObjectSomeValuesFrom(<http://www.ontologydesignpatterns.org/ont/dul/DUL.owl#expresses> <http://www.ontologydesignpatterns.org/ont/dul/DUL.owl#Method>))

# Class: <http://www.ease-crc.org/ont/SOMA-PYCRAM.owl#PyCramActionDesignatorReferenet> (PyCRAM Action Designator Referent)

AnnotationAssertion(rdfs:comment <http://www.ease-crc.org/ont/SOMA-PYCRAM.owl#PyCramActionDesignatorReferenet> "Represents a specific description that always expands the description expressed by the 'PyCRAM Action Designator Description' of the 'PyCRAM Designator' of which this Referent is part of. This referent does not exist on all PyCRAM designators, but instead typically only on those that are the result of a 'PyCRAM Designator Resolving' task, in which a PyCRAM designator without a referent plays the role of the input and another PyCRAM designator with such a referent plays the role of the output.")
AnnotationAssertion(rdfs:label <http://www.ease-crc.org/ont/SOMA-PYCRAM.owl#PyCramActionDesignatorReferenet> "PyCRAM Action Designator Referent")
SubClassOf(<http://www.ease-crc.org/ont/SOMA-PYCRAM.owl#PyCramActionDesignatorReferenet> <http://www.ease-crc.org/ont/SOMA-PYCRAM.owl#PyCramDesignatorReferent>)
SubClassOf(<http://www.ease-crc.org/ont/SOMA-PYCRAM.owl#PyCramActionDesignatorReferenet> ObjectSomeValuesFrom(<http://www.ontologydesignpatterns.org/ont/dul/DUL.owl#expresses> ObjectIntersectionOf(<http://www.ontologydesignpatterns.org/ont/dul/DUL.owl#Plan> ObjectSomeValuesFrom(<http://www.ontologydesignpatterns.org/ont/dul/DUL.owl#expands> ObjectIntersectionOf(<http://www.ontologydesignpatterns.org/ont/dul/DUL.owl#Method> ObjectSomeValuesFrom(<http://www.ontologydesignpatterns.org/ont/dul/DUL.owl#isExpressedBy> <http://www.ease-crc.org/ont/SOMA-PYCRAM.owl#PyCramActionDesignatorDescription>))))))

# Class: <http://www.ease-crc.org/ont/SOMA-PYCRAM.owl#PyCramDesignatorDescription> (PyCRAM Designator Description)

AnnotationAssertion(rdfs:comment <http://www.ease-crc.org/ont/SOMA-PYCRAM.owl#PyCramDesignatorDescription> "The 'PyCRAM Designator Description' expresses an (underspecified) description (dul:Description) used by the CRAM framework to resolve objects, actions, motions, and locations at runtime.")
AnnotationAssertion(rdfs:label <http://www.ease-crc.org/ont/SOMA-PYCRAM.owl#PyCramDesignatorDescription> "PyCRAM Designator Description")
SubClassOf(<http://www.ease-crc.org/ont/SOMA-PYCRAM.owl#PyCramDesignatorDescription> SOMA:Structured_Text)

# Class: <http://www.ease-crc.org/ont/SOMA-PYCRAM.owl#PyCramDesignatorReferent> (PyCRAM Designator Referent)

AnnotationAssertion(rdfs:comment <http://www.ease-crc.org/ont/SOMA-PYCRAM.owl#PyCramDesignatorReferent> "Represents a specific description that always expands the description expressed by the 'PyCRAM Designator Description' of the 'PyCRAM Designator' of which this Referent is part of. This referent does not exist on all PyCRAM designators, but instead typically only on those that are the result of a 'PyCRAM Designator Resolving' task, in which a PyCRAM designator without a referent plays the role of the input and another PyCRAM designator with such a referent plays the role of the output.")
AnnotationAssertion(rdfs:label <http://www.ease-crc.org/ont/SOMA-PYCRAM.owl#PyCramDesignatorReferent> "PyCRAM Designator Referent")
SubClassOf(<http://www.ease-crc.org/ont/SOMA-PYCRAM.owl#PyCramDesignatorReferent> SOMA:Structured_Text)

# Class: <http://www.ease-crc.org/ont/SOMA-PYCRAM.owl#PyCramLocationDesignator> (PyCRAM Location Designator)

AnnotationAssertion(rdfs:comment <http://www.ease-crc.org/ont/SOMA-PYCRAM.owl#PyCramLocationDesignator> "A 'PyCram Designator' that has the components of a 'PyCRAM Location Designator Description' that expresses a 'Description' of a 'Physical Place' and, possibly if it is the output of a' PyCRAM Designator Resolving' task, a 'PyCRAM Location Designator Referent' that expands the first expressed description to a more concrete Description of a 'Physical place'.")
AnnotationAssertion(rdfs:label <http://www.ease-crc.org/ont/SOMA-PYCRAM.owl#PyCramLocationDesignator> "PyCRAM Location Designator")
SubClassOf(<http://www.ease-crc.org/ont/SOMA-PYCRAM.owl#PyCramLocationDesignator> SOMA:PyCramDesignator)
SubClassOf(<http://www.ease-crc.org/ont/SOMA-PYCRAM.owl#PyCramLocationDesignator> ObjectSomeValuesFrom(<http://www.ontologydesignpatterns.org/ont/dul/DUL.owl#hasProperPart> <http://www.ease-crc.org/ont/SOMA-PYCRAM.owl#PyCramLocationDesignatorDescription>))

# Class: <http://www.ease-crc.org/ont/SOMA-PYCRAM.owl#PyCramLocationDesignatorDescription> (PyCRAM Location Designator Description)

AnnotationAssertion(rdfs:comment <http://www.ease-crc.org/ont/SOMA-PYCRAM.owl#PyCramLocationDesignatorDescription> "Expresses an (underspecified) description (dul:Description) used by the CRAM framework to resolve locations at runtime.")
AnnotationAssertion(rdfs:label <http://www.ease-crc.org/ont/SOMA-PYCRAM.owl#PyCramLocationDesignatorDescription> "PyCRAM Location Designator Description")
SubClassOf(<http://www.ease-crc.org/ont/SOMA-PYCRAM.owl#PyCramLocationDesignatorDescription> <http://www.ease-crc.org/ont/SOMA-PYCRAM.owl#PyCramDesignatorDescription>)
SubClassOf(<http://www.ease-crc.org/ont/SOMA-PYCRAM.owl#PyCramLocationDesignatorDescription> ObjectSomeValuesFrom(<http://www.ontologydesignpatterns.org/ont/dul/DUL.owl#expresses> ObjectIntersectionOf(<http://www.ontologydesignpatterns.org/ont/dul/DUL.owl#Description> ObjectSomeValuesFrom(<http://www.ontologydesignpatterns.org/ont/dul/DUL.owl#describes> <http://www.ontologydesignpatterns.org/ont/dul/DUL.owl#PhysicalPlace>))))

# Class: <http://www.ease-crc.org/ont/SOMA-PYCRAM.owl#PyCramLocationDesignatorReferenet> (PyCRAM Location Designator Referent)

AnnotationAssertion(rdfs:comment <http://www.ease-crc.org/ont/SOMA-PYCRAM.owl#PyCramLocationDesignatorReferenet> "Represents a specific description that always expands the description expressed by the 'PyCRAM Location Designator Description' of the 'PyCRAM Designator' of which this Referent is part of. This referent does not exist on all PyCRAM designators, but instead typically only on those that are the result of a 'PyCRAM Designator Resolving' task, in which a PyCRAM designator without a referent plays the role of the input and another PyCRAM designator with such a referent plays the role of the output.")
AnnotationAssertion(rdfs:label <http://www.ease-crc.org/ont/SOMA-PYCRAM.owl#PyCramLocationDesignatorReferenet> "PyCRAM Location Designator Referent")
SubClassOf(<http://www.ease-crc.org/ont/SOMA-PYCRAM.owl#PyCramLocationDesignatorReferenet> <http://www.ease-crc.org/ont/SOMA-PYCRAM.owl#PyCramDesignatorReferent>)
SubClassOf(<http://www.ease-crc.org/ont/SOMA-PYCRAM.owl#PyCramLocationDesignatorReferenet> ObjectSomeValuesFrom(<http://www.ontologydesignpatterns.org/ont/dul/DUL.owl#expresses> ObjectIntersectionOf(<http://www.ontologydesignpatterns.org/ont/dul/DUL.owl#Description> ObjectSomeValuesFrom(<http://www.ontologydesignpatterns.org/ont/dul/DUL.owl#describes> <http://www.ontologydesignpatterns.org/ont/dul/DUL.owl#PhysicalPlace>) ObjectSomeValuesFrom(<http://www.ontologydesignpatterns.org/ont/dul/DUL.owl#expands> ObjectIntersectionOf(<http://www.ontologydesignpatterns.org/ont/dul/DUL.owl#Description> ObjectSomeValuesFrom(<http://www.ontologydesignpatterns.org/ont/dul/DUL.owl#isExpressedBy> <http://www.ease-crc.org/ont/SOMA-PYCRAM.owl#PyCramActionDesignatorDescription>))))))

# Class: <http://www.ease-crc.org/ont/SOMA-PYCRAM.owl#PyCramMotionDesignatorDescription> (PyCRAM Motion Designator Description)

AnnotationAssertion(rdfs:comment <http://www.ease-crc.org/ont/SOMA-PYCRAM.owl#PyCramMotionDesignatorDescription> "Expresses an (underspecified) description (dul:Description) used by the CRAM framework to resolve motions at runtime.")
AnnotationAssertion(rdfs:label <http://www.ease-crc.org/ont/SOMA-PYCRAM.owl#PyCramMotionDesignatorDescription> "PyCRAM Motion Designator Description")
SubClassOf(<http://www.ease-crc.org/ont/SOMA-PYCRAM.owl#PyCramMotionDesignatorDescription> <http://www.ease-crc.org/ont/SOMA-PYCRAM.owl#PyCramDesignatorDescription>)
SubClassOf(<http://www.ease-crc.org/ont/SOMA-PYCRAM.owl#PyCramMotionDesignatorDescription> ObjectSomeValuesFrom(<http://www.ontologydesignpatterns.org/ont/dul/DUL.owl#expresses> SOMA:MotionDescription))

# Class: <http://www.ease-crc.org/ont/SOMA-PYCRAM.owl#PyCramMotionDesignatorReferenet> (PyCRAM Motion Designator Referent)

AnnotationAssertion(rdfs:comment <http://www.ease-crc.org/ont/SOMA-PYCRAM.owl#PyCramMotionDesignatorReferenet> "Represents a specific description that always expands the description expressed by the 'PyCRAM Motion Designator Description' of the 'PyCRAM Designator' of which this Referent is part of. This referent does not exist on all PyCRAM designators, but instead typically only on those that are the result of a 'PyCRAM Designator Resolving' task, in which a PyCRAM designator without a referent plays the role of the input and another PyCRAM designator with such a referent plays the role of the output.")
AnnotationAssertion(rdfs:label <http://www.ease-crc.org/ont/SOMA-PYCRAM.owl#PyCramMotionDesignatorReferenet> "PyCRAM Motion Designator Referent")
SubClassOf(<http://www.ease-crc.org/ont/SOMA-PYCRAM.owl#PyCramMotionDesignatorReferenet> <http://www.ease-crc.org/ont/SOMA-PYCRAM.owl#PyCramDesignatorReferent>)
SubClassOf(<http://www.ease-crc.org/ont/SOMA-PYCRAM.owl#PyCramMotionDesignatorReferenet> ObjectSomeValuesFrom(<http://www.ontologydesignpatterns.org/ont/dul/DUL.owl#expresses> ObjectIntersectionOf(SOMA:MotionDescription ObjectSomeValuesFrom(<http://www.ontologydesignpatterns.org/ont/dul/DUL.owl#expands> ObjectIntersectionOf(SOMA:MotionDescription ObjectSomeValuesFrom(<http://www.ontologydesignpatterns.org/ont/dul/DUL.owl#isExpressedBy> <http://www.ease-crc.org/ont/SOMA-PYCRAM.owl#PyCramMotionDesignatorDescription>))))))

# Class: <http://www.ease-crc.org/ont/SOMA-PYCRAM.owl#PyCramObjectDesignatorDescription> (PyCRAM Object Designator Description)

AnnotationAssertion(rdfs:comment <http://www.ease-crc.org/ont/SOMA-PYCRAM.owl#PyCramObjectDesignatorDescription> "Expresses an (underspecified) description (dul:Description) used by the CRAM framework to resolve physical artifacts at runtime.")
AnnotationAssertion(rdfs:label <http://www.ease-crc.org/ont/SOMA-PYCRAM.owl#PyCramObjectDesignatorDescription> "PyCRAM Object Designator Description")
SubClassOf(<http://www.ease-crc.org/ont/SOMA-PYCRAM.owl#PyCramObjectDesignatorDescription> <http://www.ease-crc.org/ont/SOMA-PYCRAM.owl#PyCramDesignatorDescription>)
SubClassOf(<http://www.ease-crc.org/ont/SOMA-PYCRAM.owl#PyCramObjectDesignatorDescription> ObjectSomeValuesFrom(<http://www.ontologydesignpatterns.org/ont/dul/DUL.owl#expresses> ObjectIntersectionOf(<http://www.ontologydesignpatterns.org/ont/dul/DUL.owl#Description> ObjectSomeValuesFrom(<http://www.ontologydesignpatterns.org/ont/dul/DUL.owl#describes> <http://www.ontologydesignpatterns.org/ont/dul/DUL.owl#PhysicalArtifact>))))

# Class: <http://www.ease-crc.org/ont/SOMA-PYCRAM.owl#PyCramObjectDesignatorReferenet> (PyCRAM Object Designator Referent)

AnnotationAssertion(rdfs:comment <http://www.ease-crc.org/ont/SOMA-PYCRAM.owl#PyCramObjectDesignatorReferenet> "Represents a specific description that always expands the description expressed by the 'PyCRAM Object Designator Description' of the 'PyCRAM Designator' of which this Referent is part of. This referent does not exist on all PyCRAM designators, but instead typically only on those that are the result of a 'PyCRAM Designator Resolving' task, in which a PyCRAM designator without a referent plays the role of the input and another PyCRAM designator with such a referent plays the role of the output.")
AnnotationAssertion(rdfs:label <http://www.ease-crc.org/ont/SOMA-PYCRAM.owl#PyCramObjectDesignatorReferenet> "PyCRAM Object Designator Referent")
SubClassOf(<http://www.ease-crc.org/ont/SOMA-PYCRAM.owl#PyCramObjectDesignatorReferenet> <http://www.ease-crc.org/ont/SOMA-PYCRAM.owl#PyCramDesignatorReferent>)
SubClassOf(<http://www.ease-crc.org/ont/SOMA-PYCRAM.owl#PyCramObjectDesignatorReferenet> ObjectSomeValuesFrom(<http://www.ontologydesignpatterns.org/ont/dul/DUL.owl#expresses> ObjectIntersectionOf(<http://www.ontologydesignpatterns.org/ont/dul/DUL.owl#Description> ObjectSomeValuesFrom(<http://www.ontologydesignpatterns.org/ont/dul/DUL.owl#describes> <http://www.ontologydesignpatterns.org/ont/dul/DUL.owl#PhysicalArtifact>) ObjectSomeValuesFrom(<http://www.ontologydesignpatterns.org/ont/dul/DUL.owl#expands> ObjectIntersectionOf(<http://www.ontologydesignpatterns.org/ont/dul/DUL.owl#Description> ObjectSomeValuesFrom(<http://www.ontologydesignpatterns.org/ont/dul/DUL.owl#isExpressedBy> <http://www.ease-crc.org/ont/SOMA-PYCRAM.owl#PyCramObjectDesignatorDescription>))))))

# Class: SOMA:PyCramActionDesignator (PyCRAM Action Designator)

AnnotationAssertion(rdfs:comment SOMA:PyCramActionDesignator "A 'PyCram Designator' that has the components of a 'PyCRAM Action Designator Description' that expresses a 'Method' describing how to perform some complex 'Task' and, possibly if it is the output of a' PyCRAM Designator Resolving' task, a 'PyCRAM Action Designator Referent' that expands the first expressed description to a more concrete 'Plan'.")
AnnotationAssertion(rdfs:label SOMA:PyCramActionDesignator "PyCRAM Action Designator")
SubClassOf(SOMA:PyCramActionDesignator SOMA:PyCramDesignator)
SubClassOf(SOMA:PyCramActionDesignator ObjectSomeValuesFrom(<http://www.ontologydesignpatterns.org/ont/dul/DUL.owl#hasProperPart> <http://www.ease-crc.org/ont/SOMA-PYCRAM.owl#PyCramActionDesignatorDescription>))

# Class: SOMA:PyCramDesignator (PyCRAM Designator)

AnnotationAssertion(rdfs:comment SOMA:PyCramDesignator "A PyCRAM designator is a structured data object (possibly existing as a file or in memory only) with two parts:
1. The 'PyCRAM Designator Description' expresses an (underspecified) description (dul:Description) used by the CRAM framework to resolve objects, actions, motions, and locations at runtime.

2. Possibly, a 'PyCRAM Designator Referent', representing another more specific description that always expands the description expressed by the 'PyCRAM Designator Description'. This referent does not exist on all PyCRAM designators, but instead typically only on those that are the result of a 'PyCRAM Designator Resolving' task, in which a PyCRAM designator without a referent plays the role of the input and another PyCRAM designator with such a referent plays the role of the output.")
AnnotationAssertion(rdfs:label SOMA:PyCramDesignator "PyCRAM Designator")
SubClassOf(SOMA:PyCramDesignator SOMA:Structured_Text)
SubClassOf(SOMA:PyCramDesignator ObjectSomeValuesFrom(<http://www.ontologydesignpatterns.org/ont/dul/DUL.owl#expresses> <http://www.ontologydesignpatterns.org/ont/dul/DUL.owl#Description>))

# Class: SOMA:PyCramMotionDesignator (PyCRAM Motion Designator)

AnnotationAssertion(rdfs:comment SOMA:PyCramMotionDesignator "A 'PyCram Designator' that has the components of a 'PyCRAM Motion Designator Description' that expresses a 'Motion Description' and, possibly if it is the output of a' PyCRAM Designator Resolving' task, a 'PyCRAM Motion Designator Referent' that expands the first expressed description to a more concrete 'Motion Description'.")
AnnotationAssertion(rdfs:label SOMA:PyCramMotionDesignator "PyCRAM Motion Designator")
SubClassOf(SOMA:PyCramMotionDesignator SOMA:PyCramDesignator)
SubClassOf(SOMA:PyCramMotionDesignator ObjectSomeValuesFrom(<http://www.ontologydesignpatterns.org/ont/dul/DUL.owl#expresses> SOMA:MotionDescription))
SubClassOf(SOMA:PyCramMotionDesignator ObjectSomeValuesFrom(<http://www.ontologydesignpatterns.org/ont/dul/DUL.owl#hasProperPart> <http://www.ease-crc.org/ont/SOMA-PYCRAM.owl#PyCramMotionDesignatorDescription>))

# Class: SOMA:PyCramObjectDesignator (PyCRAM Object Designator)

AnnotationAssertion(rdfs:comment SOMA:PyCramObjectDesignator "A 'PyCram Designator' that has the components of a 'PyCRAM Object Designator Description' that expresses a 'Description' of a 'Physical artifact' and, possibly if it is the output of a' PyCRAM Designator Resolving' task, a 'PyCRAM Object Designator Referent' that expands the first expressed description to a more concrete Description of a 'Physical artifact'.")
AnnotationAssertion(rdfs:label SOMA:PyCramObjectDesignator "PyCRAM Object Designator")
SubClassOf(SOMA:PyCramObjectDesignator SOMA:PyCramDesignator)
SubClassOf(SOMA:PyCramObjectDesignator ObjectSomeValuesFrom(<http://www.ontologydesignpatterns.org/ont/dul/DUL.owl#hasProperPart> <http://www.ease-crc.org/ont/SOMA-PYCRAM.owl#PyCramObjectDesignatorDescription>))

# Class: SOMA:Resolving_of_PyCRAM_Designators (Resolving a PyCRAM Designator)

AnnotationAssertion(rdfs:label SOMA:Resolving_of_PyCRAM_Designators "Resolving a PyCRAM Designator")
SubClassOf(SOMA:Resolving_of_PyCRAM_Designators SOMA:DerivingInformation)
SubClassOf(SOMA:Resolving_of_PyCRAM_Designators ObjectSomeValuesFrom(SOMA:isTaskOfInputRole ObjectIntersectionOf(SOMA:Premise ObjectSomeValuesFrom(<http://www.ontologydesignpatterns.org/ont/dul/DUL.owl#isRoleOf> SOMA:PyCramDesignator))))
SubClassOf(SOMA:Resolving_of_PyCRAM_Designators ObjectSomeValuesFrom(SOMA:isTaskOfOutputRole ObjectIntersectionOf(SOMA:Conclusion ObjectSomeValuesFrom(<http://www.ontologydesignpatterns.org/ont/dul/DUL.owl#isRoleOf> SOMA:PyCramDesignator))))


)