Prefix(:=<http://www.ease-crc.org/ont/SOMA-NEEM.owl#>)
Prefix(dc:=<http://purl.org/dc/elements/1.1/>)
Prefix(owl:=<http://www.w3.org/2002/07/owl#>)
Prefix(rdf:=<http://www.w3.org/1999/02/22-rdf-syntax-ns#>)
Prefix(xml:=<http://www.w3.org/XML/1998/namespace>)
Prefix(xsd:=<http://www.w3.org/2001/XMLSchema#>)
Prefix(SOMA:=<http://www.ease-crc.org/ont/SOMA.owl#>)
Prefix(rdfs:=<http://www.w3.org/2000/01/rdf-schema#>)


Ontology(<http://www.ease-crc.org/ont/SOMA-NEEM.owl>
Import(<http://www.ease-crc.org/ont/SOMA.owl>)
Annotation(rdfs:comment "SOMA-NEEM.owl defines concepts useful to describe metadata associated to a NEEM, such as the recorded media that it includes.")

Declaration(Class(SOMA:KinoDynamicData))
Declaration(Class(SOMA:MeshShapeData))
Declaration(Class(SOMA:VideoData))



############################
#   Classes
############################

# Class: SOMA:KinoDynamicData (Kino-dynamic data)

AnnotationAssertion(rdfs:comment SOMA:KinoDynamicData "An InformationObject containing data about how a physical object is put together such that its parts may move relative to each other, and what the physical characteristics of those parts are.")
AnnotationAssertion(rdfs:label SOMA:KinoDynamicData "Kino-dynamic data"@en)
SubClassOf(SOMA:KinoDynamicData <http://www.ontologydesignpatterns.org/ont/dul/DUL.owl#InformationObject>)
SubClassOf(SOMA:KinoDynamicData ObjectAllValuesFrom(<http://www.ontologydesignpatterns.org/ont/dul/DUL.owl#isAbout> <http://www.ontologydesignpatterns.org/ont/dul/DUL.owl#PhysicalObject>))

# Class: SOMA:MeshShapeData (Mesh-shape data)

AnnotationAssertion(rdfs:comment SOMA:MeshShapeData "An InformationObject containing data about the geometry of a physical object.")
AnnotationAssertion(rdfs:label SOMA:MeshShapeData "Mesh-shape data"@en)
SubClassOf(SOMA:MeshShapeData <http://www.ontologydesignpatterns.org/ont/dul/DUL.owl#InformationObject>)
SubClassOf(SOMA:MeshShapeData ObjectAllValuesFrom(<http://www.ontologydesignpatterns.org/ont/dul/DUL.owl#isAbout> <http://www.ontologydesignpatterns.org/ont/dul/DUL.owl#PhysicalObject>))

# Class: SOMA:VideoData (Video data)

AnnotationAssertion(rdfs:comment SOMA:VideoData "An information object containing data for audio-visual modalities.")
AnnotationAssertion(rdfs:label SOMA:VideoData "Video data"@en)
SubClassOf(SOMA:VideoData <http://www.ontologydesignpatterns.org/ont/dul/DUL.owl#InformationObject>)


)