Prefix(:=<http://www.ease-crc.org/ont/SOMA-ELAN.owl#>)
Prefix(dc:=<http://purl.org/dc/elements/1.1/>)
Prefix(owl:=<http://www.w3.org/2002/07/owl#>)
Prefix(rdf:=<http://www.w3.org/1999/02/22-rdf-syntax-ns#>)
Prefix(xml:=<http://www.w3.org/XML/1998/namespace>)
Prefix(xsd:=<http://www.w3.org/2001/XMLSchema#>)
Prefix(SOMA:=<http://www.ease-crc.org/ont/SOMA.owl#>)
Prefix(rdfs:=<http://www.w3.org/2000/01/rdf-schema#>)


Ontology(<http://www.ease-crc.org/ont/SOMA-ELAN.owl>
Import(<http://www.ease-crc.org/ont/SOMA-ACT.owl>)
Annotation(rdfs:comment "SOMA-ELAN.owl is chiefly concerned with providing a controlled vocabulary for annotations of human activity episodes coming from the area H subprojects of the EASE CRC.

SOMA-ELAN.owl should at least import SOMA-ACT.owl and therefore indirectly imports all other modules that SOMA-ACT depends on. This is because the controlled vocabulary is defined as alternative labels for concepts defined in the various modules of SOMA.")

Declaration(Class(SOMA:PrepareForBreakfast))
Declaration(Class(SOMA:PrepareForDinner))
Declaration(Class(SOMA:PrepareForLunch))
Declaration(Class(SOMA:PrepareForMeal))
Declaration(Class(SOMA:SettingTheTable))
Declaration(DataProperty(SOMA:expectedNumberOfPeople))
Declaration(DataProperty(SOMA:formalityLevel))
Declaration(AnnotationProperty(SOMA:ELANName))
Declaration(AnnotationProperty(SOMA:ELANUsageGuideline))
Declaration(AnnotationProperty(SOMA:UsageGuideline))
Declaration(AnnotationProperty(SOMA:nickname))
############################
#   Annotation Properties
############################

# Annotation Property: SOMA:ELANName (SOMA:ELANName)

AnnotationAssertion(rdfs:comment SOMA:ELANName "If present, used by the controlled vocabulary generation script to create a vocabulary entry. By default, the concept name itself is used for the vocabulary entry.")
SubAnnotationPropertyOf(SOMA:ELANName SOMA:nickname)

# Annotation Property: SOMA:ELANUsageGuideline (SOMA:ELANUsageGuideline)

AnnotationAssertion(rdfs:comment SOMA:ELANUsageGuideline "Provides a short description, similar to a definition, of a controlled vocabulary entry for ELAN.")
SubAnnotationPropertyOf(SOMA:ELANUsageGuideline SOMA:UsageGuideline)



############################
#   Data Properties
############################

# Data Property: SOMA:expectedNumberOfPeople (SOMA:expectedNumberOfPeople)

AnnotationAssertion(rdfs:comment SOMA:expectedNumberOfPeople "Used by the description of a task that classifies some event, usually a social gathering such as a meal, or by a description of a task to prepare for such an event, to record the number of people expected to participate.")
SubDataPropertyOf(SOMA:expectedNumberOfPeople <http://www.ontologydesignpatterns.org/ont/dul/DUL.owl#hasDataValue>)
DataPropertyDomain(SOMA:expectedNumberOfPeople ObjectIntersectionOf(<http://www.ontologydesignpatterns.org/ont/dul/DUL.owl#Description> ObjectSomeValuesFrom(<http://www.ontologydesignpatterns.org/ont/dul/DUL.owl#defines> <http://www.ontologydesignpatterns.org/ont/dul/DUL.owl#Task>)))
DataPropertyRange(SOMA:expectedNumberOfPeople xsd:integer)

# Data Property: SOMA:formalityLevel (SOMA:formalityLevel)

AnnotationAssertion(rdfs:comment SOMA:formalityLevel "Records the formality level in a description associated to some event, usually a social gathering such as a meal.

The association between the Description and the Event can be direct (the Description is about the Event itself) but it can also be indirect in various ways. A typical example of the latter is where the Description is a Goal for a Task to prepare for the Event in question, as when the Goal of a SettingTheTable task would record the formality level of a meal, which will occur at some point after the task completes.")
SubDataPropertyOf(SOMA:formalityLevel <http://www.ontologydesignpatterns.org/ont/dul/DUL.owl#hasDataValue>)
DataPropertyDomain(SOMA:formalityLevel ObjectIntersectionOf(<http://www.ontologydesignpatterns.org/ont/dul/DUL.owl#Description> ObjectSomeValuesFrom(<http://www.ontologydesignpatterns.org/ont/dul/DUL.owl#defines> <http://www.ontologydesignpatterns.org/ont/dul/DUL.owl#Task>)))
DataPropertyRange(SOMA:formalityLevel xsd:string)



############################
#   Classes
############################

# Class: SOMA:Arranging (SOMA:Arranging)

AnnotationAssertion(SOMA:ELANName SOMA:Arranging "construction-arrange-objects")
AnnotationAssertion(SOMA:ELANUsageGuideline SOMA:Arranging "A task involving the arrangement of a collection of objects in a particular way.")

# Class: SOMA:PrepareForBreakfast (SOMA:PrepareForBreakfast)

AnnotationAssertion(rdfs:comment SOMA:PrepareForBreakfast "Describes a goal to prepare a table or dining area for a breakfast.")
SubClassOf(SOMA:PrepareForBreakfast SOMA:PrepareForMeal)

# Class: SOMA:PrepareForDinner (SOMA:PrepareForDinner)

AnnotationAssertion(rdfs:comment SOMA:PrepareForDinner "Describes a goal to prepare a table or dining area for a dinner.")
SubClassOf(SOMA:PrepareForDinner SOMA:PrepareForMeal)

# Class: SOMA:PrepareForLunch (SOMA:PrepareForLunch)

AnnotationAssertion(rdfs:comment SOMA:PrepareForLunch "Describes a goal to prepare a table or dining area for a lunch.")
SubClassOf(SOMA:PrepareForLunch SOMA:PrepareForMeal)

# Class: SOMA:PrepareForMeal (SOMA:PrepareForMeal)

AnnotationAssertion(rdfs:comment SOMA:PrepareForMeal "A description of a goal to prepare for serving a meal by setting a table.

The meal will have a number of expected participants and a level of formality.")
SubClassOf(SOMA:PrepareForMeal <http://www.ontologydesignpatterns.org/ont/dul/DUL.owl#Goal>)
SubClassOf(SOMA:PrepareForMeal DataSomeValuesFrom(SOMA:expectedNumberOfPeople xsd:integer))
SubClassOf(SOMA:PrepareForMeal DataSomeValuesFrom(SOMA:formalityLevel xsd:boolean))

# Class: SOMA:SettingTheTable (SOMA:SettingTheTable)

AnnotationAssertion(rdfs:comment SOMA:SettingTheTable "The task to prepare a table for a meal.")
SubClassOf(SOMA:SettingTheTable SOMA:Arranging)
SubClassOf(SOMA:SettingTheTable ObjectSomeValuesFrom(<http://www.ontologydesignpatterns.org/ont/dul/DUL.owl#isTaskDefinedIn> SOMA:PrepareForMeal))


AnnotationAssertion(SOMA:ELANName SOMA:Actuating "move-object")
AnnotationAssertion(SOMA:ELANUsageGuideline SOMA:Actuating "Superconcept for the Agent moving some (usually, but not always, grasped) object; use more specific labels where appropriate.")
AnnotationAssertion(SOMA:ELANName SOMA:Approaching "move-body-walk-to")
AnnotationAssertion(SOMA:ELANUsageGuideline SOMA:Approaching "walk (to a location, or in a direction)")
AnnotationAssertion(SOMA:ELANName SOMA:AreaSurveying "perception-survey-area")
AnnotationAssertion(SOMA:ELANUsageGuideline SOMA:AreaSurveying "Visually survey an area, for objects or potential object positions.")
AnnotationAssertion(SOMA:ELANName SOMA:Assembling "construction-assembly")
AnnotationAssertion(SOMA:ELANUsageGuideline SOMA:Assembling "A task involving the putting together of objects to form an assembly, usually in a way in which these objects can be recovered.")
AnnotationAssertion(SOMA:ELANName SOMA:BodyMovement "move-body-general")
AnnotationAssertion(SOMA:ELANUsageGuideline SOMA:BodyMovement "The Agent moves its body in some way. Use more specific labels where appropriate.")
AnnotationAssertion(SOMA:ELANName SOMA:Catching "move-object-catch")
AnnotationAssertion(SOMA:ELANUsageGuideline SOMA:Catching "Agent intercepts and arrests the motion of an object.")
AnnotationAssertion(SOMA:ELANName SOMA:Closing "move-object-close")
AnnotationAssertion(SOMA:ELANUsageGuideline SOMA:Closing "Move an object so that it no longer exposes an interior surface.")
AnnotationAssertion(SOMA:ELANName SOMA:Constructing "construction-general")
AnnotationAssertion(SOMA:ELANUsageGuideline SOMA:Constructing "Superconcept for tasks requiring the creation of some object (including an arrangement or collection of objects); use more specific labels where appropriate")
AnnotationAssertion(SOMA:ELANName SOMA:Cutting "object-modification-cutting")
AnnotationAssertion(SOMA:ELANUsageGuideline SOMA:Cutting "A task that requires some object to be cut into pieces. The cut is often irreversible.")
AnnotationAssertion(SOMA:ELANName SOMA:Dicing "object-modification-dicing")
AnnotationAssertion(SOMA:ELANUsageGuideline SOMA:Dicing "A task that requires an object to be (at least partially) cut into slices.")
AnnotationAssertion(SOMA:ELANName SOMA:Distancing "move-body-walk-backaway")
AnnotationAssertion(SOMA:ELANUsageGuideline SOMA:Distancing "walk (away from a location, in a direction)")
AnnotationAssertion(SOMA:ELANName SOMA:Dropping "move-object-drop")
AnnotationAssertion(SOMA:ELANUsageGuideline SOMA:Dropping "Agent undoes whatever functional control they have on an object, but without imparting significant momentum to it, and allows the object to fall under the influence of gravity.")
AnnotationAssertion(SOMA:ELANName SOMA:EndEffectorPositioning "manipulation-hand-positioning")
AnnotationAssertion(SOMA:ELANUsageGuideline SOMA:EndEffectorPositioning "Superconcept for the Agent moving their arm(s) to positioning their hand/end effector; use more specific labels where appropriate.")
AnnotationAssertion(SOMA:ELANName SOMA:GraspTransfer "move-hand-grasp-transfer")
AnnotationAssertion(SOMA:ELANUsageGuideline SOMA:GraspTransfer "have grasped an object with one hand, now grasp it with the other and release it from the first")
AnnotationAssertion(SOMA:ELANName SOMA:Grasping "manipulation-grasp")
AnnotationAssertion(SOMA:ELANUsageGuideline SOMA:Grasping "Agent grasps an object.")
AnnotationAssertion(SOMA:ELANName SOMA:HeadMovement "move-head")
AnnotationAssertion(SOMA:ELANUsageGuideline SOMA:HeadMovement "Superconcept for the Agent moving their head; use more specific labels where appropriate.")
AnnotationAssertion(SOMA:ELANName SOMA:HeadTurning "move-head-turn")
AnnotationAssertion(SOMA:ELANUsageGuideline SOMA:HeadTurning "Turn head (e.g. for visual search).")
AnnotationAssertion(SOMA:ELANName SOMA:Holding "move-object-hold")
AnnotationAssertion(SOMA:ELANUsageGuideline SOMA:Holding "Have grasped an object with hand, and move it while held.")
AnnotationAssertion(SOMA:ELANName SOMA:Leaning "move-body-lean")
AnnotationAssertion(SOMA:ELANUsageGuideline SOMA:Leaning "move, bending, with torso in a specific direction")
AnnotationAssertion(SOMA:ELANName SOMA:Lifting "move-object-lift")
AnnotationAssertion(SOMA:ELANUsageGuideline SOMA:Lifting "Having grasped an object with their hand, the agent now lifts it from the supporting surface.")
AnnotationAssertion(SOMA:ELANName SOMA:Locomotion "move-body-locomotion")
AnnotationAssertion(SOMA:ELANUsageGuideline SOMA:Locomotion "Superconcept for the Agent moving around; use more specific labels where appropriate.")
AnnotationAssertion(SOMA:ELANName SOMA:LookingFor "perception-search-for-object")
AnnotationAssertion(SOMA:ELANUsageGuideline SOMA:LookingFor "The agent searches, usually visually, for the location, or a possible new location, of an object")
AnnotationAssertion(SOMA:ELANName SOMA:Lowering "move-object-lower")
AnnotationAssertion(SOMA:ELANUsageGuideline SOMA:Lowering "The agent lowers a, usually held in hand(s), object.")
AnnotationAssertion(SOMA:ELANName SOMA:Manipulating "manipulation-general")
AnnotationAssertion(SOMA:ELANUsageGuideline SOMA:Manipulating "These are Actions in which the Agent exerts or prepares to exert some influence over some other participant Phyiscal Objects by way of its prehensile body parts (usually, hands).")
AnnotationAssertion(SOMA:ELANName SOMA:MetaCognitionEvaluationTopic "ta-meta-cognition-evaluation")
AnnotationAssertion(SOMA:ELANUsageGuideline SOMA:MetaCognitionEvaluationTopic "an agent analyzes and describes the process by which they evaluate whether/to what a extent a goal was reached")
AnnotationAssertion(SOMA:ELANName SOMA:MetaCognitionMemoryTopic "ta-meta-cognition-memory")
AnnotationAssertion(SOMA:ELANUsageGuideline SOMA:MetaCognitionMemoryTopic "an agent describes how and/or why they (failed to) memorize something")
AnnotationAssertion(SOMA:ELANName SOMA:MetaCognitionPlanningTopic "ta-meta-cognition-planning")
AnnotationAssertion(SOMA:ELANUsageGuideline SOMA:MetaCognitionPlanningTopic "an agent analyzes and describes the process they use to plan their behavior")
AnnotationAssertion(SOMA:ELANName SOMA:MetaCognitionTopic "ta-meta-cognition")
AnnotationAssertion(SOMA:ELANUsageGuideline SOMA:MetaCognitionTopic "Superconcept for cases where the agent describes the results of analyzing their own thought processes; use more specific labels where appropriate.")
AnnotationAssertion(SOMA:ELANName SOMA:Mixing "construction-mixing")
AnnotationAssertion(SOMA:ELANUsageGuideline SOMA:Mixing "A task involving the putting together of several objects, which are thereafter not recoverable.")
AnnotationAssertion(SOMA:ELANName SOMA:ModifyingPhysicalObject "object-modification-general")
AnnotationAssertion(SOMA:ELANUsageGuideline SOMA:ModifyingPhysicalObject "Superconcept for tasks involving the changing of the state some object(s) is/are in; use more specific labels where appropriate.")
AnnotationAssertion(SOMA:ELANName SOMA:MovingAway "move-body-walk-backaway")
AnnotationAssertion(SOMA:ELANUsageGuideline SOMA:MovingAway "walk (away from a location, in a direction)")
AnnotationAssertion(SOMA:ELANName SOMA:Opening "move-object-open")
AnnotationAssertion(SOMA:ELANUsageGuideline SOMA:Opening "Move an object so as to expose an interior surface.")
AnnotationAssertion(SOMA:ELANName SOMA:Orienting "move-object-orient")
AnnotationAssertion(SOMA:ELANUsageGuideline SOMA:Orienting "Move object to re-orient it in place on an area, or while holding.")
AnnotationAssertion(SOMA:ELANName SOMA:Perceiving "perception-general")
AnnotationAssertion(SOMA:ELANUsageGuideline SOMA:Perceiving "Superconcept for perception tasks. Use more specific levels where appropriate.")
AnnotationAssertion(SOMA:ELANName SOMA:PhysicalAcquiring "physically-acquire-object")
AnnotationAssertion(SOMA:ELANUsageGuideline SOMA:PhysicalAcquiring "Superconcept for tasks requiring that an object be put in such a physical state so that it is usable/available for other tasks.")
AnnotationAssertion(SOMA:ELANUsageGuideline SOMA:PhysicalAction "Superconcept for the Agent doing something with their hands/end effectors; use more specific labels where appropriate.")
AnnotationAssertion(SOMA:ELANName SOMA:PickingUp "move-object-pick-up")
AnnotationAssertion(SOMA:ELANUsageGuideline SOMA:PickingUp "Agent grasps an object and removes it from its previous location.")
AnnotationAssertion(SOMA:ELANName SOMA:Positioning "move-object-positioning")
AnnotationAssertion(SOMA:ELANUsageGuideline SOMA:Positioning "Move an object so that it has a particular pose.")
AnnotationAssertion(SOMA:ELANName SOMA:PosturalMoving "move-body-posture")
AnnotationAssertion(SOMA:ELANUsageGuideline SOMA:PosturalMoving "Superconcept for motions where the Agent changes posture; use more specific labels where appropriate.")
AnnotationAssertion(SOMA:ELANName SOMA:Pushing "move-object-push")
AnnotationAssertion(SOMA:ELANUsageGuideline SOMA:Pushing "Superconcept for the Agent exerting force on an object to push it; use more specific labels where appropriate.")
AnnotationAssertion(SOMA:ELANName SOMA:PushingAway "move-object-push-away")
AnnotationAssertion(SOMA:ELANUsageGuideline SOMA:PushingAway "Agent exerts force on an object to move it away from themselves.")
AnnotationAssertion(SOMA:ELANName SOMA:PushingDown "move-object-push-down")
AnnotationAssertion(SOMA:ELANUsageGuideline SOMA:PushingDown "Exert force on an object to move it in some functionally meaningful direction, such as pushing down a button (even when the actual direction the button was pushed in was up).")
AnnotationAssertion(SOMA:ELANName SOMA:PuttingDown "manipulation-put-down")
AnnotationAssertion(SOMA:ELANUsageGuideline SOMA:PuttingDown "Agent releases their grasp on an object, but only after positioning it so that it is supported and won't fall.")
AnnotationAssertion(SOMA:ELANName SOMA:Reaching "move-hand+arm-reach")
AnnotationAssertion(SOMA:ELANUsageGuideline SOMA:Reaching "Reach arm out to prepare to grasp with hand.")
AnnotationAssertion(SOMA:ELANName SOMA:Releasing "manipulation-release")
AnnotationAssertion(SOMA:ELANUsageGuideline SOMA:Releasing "Agent releases grasp on an object.")
AnnotationAssertion(SOMA:ELANName SOMA:Retracting "move-hand+arm-retract")
AnnotationAssertion(SOMA:ELANUsageGuideline SOMA:Retracting "Draw in arm and hand toward body, and away from some object or location.")
AnnotationAssertion(SOMA:ELANName SOMA:Slicing "object-modification-slicing")
AnnotationAssertion(SOMA:ELANUsageGuideline SOMA:Slicing "A task that requires an object to be (at least partially) cut into approximately cubic pieces.")
AnnotationAssertion(SOMA:ELANName SOMA:Squeezing "move-object-squeeze")
AnnotationAssertion(SOMA:ELANUsageGuideline SOMA:Squeezing "Exert compressive force on a (usually, but not always, grasped) object.")
AnnotationAssertion(SOMA:ELANName SOMA:Standing "move-body-stand")
AnnotationAssertion(SOMA:ELANUsageGuideline SOMA:Standing "stand (at a location)")
AnnotationAssertion(SOMA:ELANName SOMA:ThinkAloudActionTopic "ta-actions")
AnnotationAssertion(SOMA:ELANUsageGuideline SOMA:ThinkAloudActionTopic "an agent describes what they are currently doing")
AnnotationAssertion(SOMA:ELANName SOMA:ThinkAloudGeneralKnowledgeTopic "ta-knowledge-general")
AnnotationAssertion(SOMA:ELANUsageGuideline SOMA:ThinkAloudGeneralKnowledgeTopic "an agent makes a statement of general knowledge, as opposed to knowledge specific to the immediate environment they are in")
AnnotationAssertion(SOMA:ELANName SOMA:ThinkAloudKnowledgeTopic "ta-knowledge")
AnnotationAssertion(SOMA:ELANUsageGuideline SOMA:ThinkAloudKnowledgeTopic "Superconcept for when an agent makes a statement of knowledge of something not immediately perceivable; use more specific labels where appropriate.")
AnnotationAssertion(SOMA:ELANName SOMA:ThinkAloudObstructionTopic "ta-issues")
AnnotationAssertion(SOMA:ELANUsageGuideline SOMA:ThinkAloudObstructionTopic "an agent describes what prevents them from undertaking some action")
AnnotationAssertion(SOMA:ELANName SOMA:ThinkAloudOpinionTopic "ta-opinions")
AnnotationAssertion(SOMA:ELANUsageGuideline SOMA:ThinkAloudOpinionTopic "an agent makes a statement of opinion")
AnnotationAssertion(SOMA:ELANName SOMA:ThinkAloudPerceptionTopic "ta-perception")
AnnotationAssertion(SOMA:ELANUsageGuideline SOMA:ThinkAloudPerceptionTopic "an agent describes what they perceive")
AnnotationAssertion(SOMA:ELANName SOMA:ThinkAloudPlanTopic "ta-plans")
AnnotationAssertion(SOMA:ELANUsageGuideline SOMA:ThinkAloudPlanTopic "an agent describes their current plan")
AnnotationAssertion(SOMA:ELANName SOMA:ThinkAloudSceneKnowledgeTopic "ta-knowledge-scene")
AnnotationAssertion(SOMA:ELANUsageGuideline SOMA:ThinkAloudSceneKnowledgeTopic "an agent makes a statement that they know something about the environment they are in, which they cannot at that moment perceive directly (but they may have perceived it earlier)")
AnnotationAssertion(SOMA:ELANName SOMA:Throwing "move-object-throw")
AnnotationAssertion(SOMA:ELANUsageGuideline SOMA:Throwing "Using its arm(s), an agent imparts momentum to a held object then releases it.")
AnnotationAssertion(SOMA:ELANName SOMA:Transporting "transport-object")
AnnotationAssertion(SOMA:ELANUsageGuideline SOMA:Transporting "A task that requires chaging the location of an object.")
AnnotationAssertion(SOMA:ELANName SOMA:Turning "move-body-turn")
AnnotationAssertion(SOMA:ELANUsageGuideline SOMA:Turning "move own body, turn")
)